fix and update notations

proof/transfer.v
@@ -18,13 +18,13 @@ Notation "s1 ;; s2" := (app s2 s1)
   (at level 58, left associativity) : subst_set_scope.
 
 Notation "s ; x : t" := (cons (pair x (sse_ev t)) s)
-  ( at level 58, x at level 0, t at level 52, left associativity) : subst_set_scope.
+  ( at level 58, x at next level, left associativity) : subst_set_scope.
 
 Notation "s ; x" := (cons (pair x sse_tv) s)
-  ( at level 58, x at level 0, left associativity) : subst_set_scope.
+  ( at level 58, left associativity) : subst_set_scope.
 
 Notation "x : t ∈ s" := (binds x (sse_ev t) s)
-   (at level 58, t at level 52, no associativity) : type_scope.
+   (at level 58, t at next level, no associativity) : type_scope.
 
 
 Fixpoint ss_to_ctx (s : subst_set) : ld_context := 
@@ -53,21 +53,23 @@ Proof.
 Qed.
 
 
+Reserved Notation "θ ⊢ t ⇝ t'"
+  (at level 65, t at next level, no associativity).
 Inductive inst_type : subst_set -> la_type -> ld_type -> Prop := 
-  | inst_t_tvar : forall θ x, wf_ss θ -> inst_type θ (la_t_tvar_f x) (ld_t_var_f x)
-  | inst_t_evar : forall θ x t, wf_ss θ -> x : t ∈ θ -> inst_type θ (la_t_evar x) t
-  | inst_t_int : forall θ, wf_ss θ -> inst_type θ la_t_int ld_t_int
+  | inst_t_tvar : forall θ x, wf_ss θ -> θ ⊢ (la_t_tvar_f x) ⇝ (ld_t_var_f x)
+  | inst_t_evar : forall θ x t, wf_ss θ -> x : t ∈ θ -> θ ⊢ (la_t_evar x) ⇝ t
+  | inst_t_int : forall θ, wf_ss θ -> θ ⊢ la_t_int ⇝ ld_t_int
   | inst_t_arrow : forall θ A' B' A B, 
-      inst_type θ A' A -> inst_type θ B' B ->
-      inst_type θ (la_t_arrow A' B') (ld_t_arrow A B)
+      θ ⊢ A' ⇝ A -> θ ⊢ B' ⇝ B ->
+      θ ⊢ (la_t_arrow A' B') ⇝ (ld_t_arrow A B)
   | inst_t_forall : forall θ L A' A,
       (forall x, x `notin` L -> 
-      inst_type θ (open_la_type_wrt_la_type A' (la_t_tvar_f x)) (open_ld_type_wrt_ld_type A (ld_t_var_f x))) ->
-      inst_type θ (la_t_forall A') (ld_t_forall A)
-.
+      θ ⊢ (open_la_type_wrt_la_type A' (la_t_tvar_f x)) ⇝ (open_ld_type_wrt_ld_type A (ld_t_var_f x))) ->
+      θ ⊢ (la_t_forall A') ⇝ (ld_t_forall A)
+where "θ ⊢ t ⇝ t'" := (inst_type θ t t').
 
 Lemma inst_t_wf_ss : forall θ t t',
-    inst_type θ t t' -> wf_ss θ.
+  θ ⊢ t ⇝ t' -> wf_ss θ.
 Proof.
   induction 1; pick fresh x'; eauto.
 Qed.
@@ -76,7 +78,7 @@ Qed.
 Inductive inst_ev : subst_set -> var -> la_typelist -> la_typelist -> Prop :=
   | inst_ev_nil : forall θ x, inst_ev θ x la_tl_nil la_tl_nil
   | inst_ev_lbs : forall θ x lb lbs ubs lb' t', inst_ev θ x lbs ubs -> 
-      inst_type θ lb lb' -> inst_type θ (la_t_evar x) t' -> ld_sub (ss_to_ctx θ) lb' t' ->inst_ev θ x (la_tl_cons lbs lb) ubs
+      inst_type θ lb lb' -> inst_type θ (la_t_evar x) t' -> ld_sub (ss_to_ctx θ) lb' t' -> inst_ev θ x (la_tl_cons lbs lb) ubs
   | inst_ev_ubs : forall θ x lbs ub ubs ub' t', inst_ev θ x lbs ubs -> 
       inst_type θ ub ub' -> inst_type θ (la_t_evar x) t' -> ld_sub (ss_to_ctx θ) t' ub' -> inst_ev θ x lbs (la_tl_cons ubs ub) 
 .
@@ -84,9 +86,11 @@ Inductive inst_ev : subst_set -> var -> la_typelist -> la_typelist -> Prop :=
 
 (* Lemma split : theta |- awl --> dwl -| theta1 -> exists theta0,  theta |- awl  *)
 
+Reserved Notation "θ ⊢ Γ ⇝ Γ' ⊣ θ'"
+  (at level 65,Γ at next level, Γ' at next level, no associativity).
 Inductive inst_worklist : subst_set -> la_worklist -> ld_worklist -> subst_set -> Prop := 
   | inst_wl_nil : forall θ, 
-      wf_ss θ -> inst_worklist θ la_wl_nil ld_wl_nil θ
+      wf_ss θ -> θ ⊢ la_wl_nil ⇝ ld_wl_nil ⊣ θ
   | inst_wl_sub : forall θ θ' awl dwl t1 t2 t1' t2', 
       inst_worklist θ awl dwl θ' -> 
       inst_type θ' t1 t1' -> 
@@ -101,7 +105,7 @@ Inductive inst_worklist : subst_set -> la_worklist -> ld_worklist -> subst_set -
       ex `notin` dom θ' -> 
       inst_ev (θ' ; ex : t) ex lbs ubs -> 
       inst_worklist θ (la_wl_cons_ev awl lbs ex ubs) dwl (θ' ; ex : t)
-.
+where "θ ⊢ Γ ⇝ Γ' ⊣ θ'" := (inst_worklist θ Γ Γ' θ').
 
 
 Definition transfer (Γ : la_worklist) (Γ' : ld_worklist) : Prop :=
