proof/completeness.v
@@ -3,7 +3,7 @@ Require Import decl.ott.
 Require Import transfer.
 
 
-Theorem completeness : forall Γ', ld_worklist_reducible Γ' -> exists Γ, transfer' Γ Γ' /\ la_worklist_reducible Γ.
+Theorem completeness : forall Γ', ld_worklist_reducible Γ' -> forall Γ, transfer' Γ Γ' /\ la_worklist_reducible Γ.
 Proof.
 Admitted.
 
