proof/soundness.v
@@ -3,23 +3,77 @@ Require Import Program.Equality.
 Require Import algo.ott.
 Require Import decl.ott.
 Require Import transfer.
+Require Import decl.properties.
 
 
-Lemma inst_forall_inv: forall t' (θ: subst_set) ex t A, inst_type (θ; ex : t) (open_la_type_wrt_la_type A (la_t_evar ex)) t' -> (exists A', inst_type θ (la_t_forall A) A').
-Proof.
-  intros. induction A.
-Admitted.
-
-
+(* https://github.com/VinaLx/dependent-worklist-inference/blob/e55fe9e7ca6b5e0538313a8cf44a57469923ca02/src-lite/transfer/properties.v#L665 *)
 (* Lemma inst_e_rev_subst' : forall v' v x Θ e'
   , lc_aexpr e'
   → x `notin` (fv_aexpr v' `union` fv_ss Θ) → Θ ⊩ v' ⇝ v
   → forall e0
   , Θ ⊩ [v' /′ x] e' ⇝ e0
   → exists e, [v /' x] e = e0 ∧ Θ ⊩ e' ⇝ e.
-Proof. *)
+Proof.
+Admitted. *)
+
+Lemma reorder: forall awl1 awl2 ex lbs ubs t m awl',
+  reorder (la_wl_app (la_wl_cons_ev awl1 lbs ex ubs) awl2) ex t m la_wl_nil awl' -> 
+  exists awl'1 awl'2, awl' = la_wl_app awl'1 awl'2.
+Admitted.
+
+Lemma inst_forall_inv: forall t' (θ: subst_set) ex t A, 
+  wf_ss θ 
+  -> inst_type (θ; ex : t) (open_la_type_wrt_la_type A (la_t_evar ex)) t' 
+  -> (exists A', inst_type θ (la_t_forall A) A').
+Proof.
+  intros. 
+  dependent induction H0. 
+  - dependent destruction A; try inversion x.
+    + exists (ld_t_forall (ld_t_var_b n)). 
+      econstructor. intros. destruct n; simpl.
+      * constructor. auto.
+      * unfold open_la_type_wrt_la_type. unfold open_ld_type_wrt_ld_type. simpl. admit.
+        (* not closed type  *)
+    + exists (ld_t_forall (ld_t_var_f x0)). econstructor. intros.
+      unfold open_la_type_wrt_la_type. unfold open_ld_type_wrt_ld_type. simpl. subst. econstructor. auto.
+  - dependent destruction A; try inversion x.
+    + destruct n; inversion x.
+      exists (ld_t_forall (ld_t_var_b 0)).
+      econstructor; intros. unfold open_la_type_wrt_la_type. unfold open_ld_type_wrt_ld_type.  simpl. econstructor. auto.
+    + subst. exists (ld_t_forall t0).
+      econstructor. intros. unfold open_la_type_wrt_la_type. unfold open_ld_type_wrt_ld_type.
+      assert (t0 = (open_ld_type_wrt_ld_type_rec 0 (ld_t_var_f x0) t0)) by admit.
+      simpl. rewrite <- H3. econstructor. subst; auto. 
+      (* need wf to ensure ex5 != ex*)
+      admit.
+  - dependent induction A; try inversion x.
+    + exists (ld_t_forall ld_t_int). admit.
+    + destruct n; inversion x.
+  - dependent destruction A; try dependent destruction x.
+    + admit. (* ** *)
+    + destruct n; inversion x. 
+  - dependent destruction A; try dependent destruction x.
+    + admit.
+    + destruct n; inversion x. 
+Admitted.
 
 
+Lemma dwl_red_ctx_wf : forall dwl, 
+  ld_worklist_reducible dwl -> ld_wf_context (ld_wl_to_ctx dwl).
+Proof.
+  induction dwl; intros; auto; 
+  dependent destruction H; auto.
+Qed.
+
+(* Lemma tl_not_empty_inv: forall tl,
+  la_tl_not_empty tl -> exists t tl', tl = la_tl_cons tl' t.
+Proof.
+  induction tl. *)
+
+
+Lemma inst_ld_type_exists: forall θ t,
+  exists t', inst_type θ t t'.
+Admitted.
 
 Theorem soundness : forall Γ, la_worklist_reducible Γ -> exists Γ', transfer Γ Γ' /\ ld_worklist_reducible Γ'.
 Proof.
@@ -27,19 +81,39 @@ Proof.
   - destruct IHla_worklist_reducible as [dwl Hdwl]. destruct Hdwl.
     exists (ld_wl_cons_tv dwl x5). split. 
     + dependent destruction H1. econstructor. econstructor. eauto.
-    + econstructor; eauto. simpl. econstructor. admit. admit.
+    + econstructor; eauto. simpl. econstructor. 
+      * now apply dwl_red_ctx_wf. 
+      * admit.
   - destruct IHla_worklist_reducible as [dwl Hdwl]. destruct Hdwl. 
     destruct tl.
     + simpl in *. exists dwl. split. 
       * unfold transfer in H1. destruct H1 as [θ'].
         exists (cons (pair ex5 (sse_ev ld_t_int)) θ'). eapply inst_wl_ev; eauto.
-        admit. constructor.
+        admit. (* * dom *)
+        constructor.
       * auto.
-    + admit.
+    + simpl in *.
+      exists dwl. destruct H1 as [θ'].
+      specialize (inst_ld_type_exists θ' t). intros. destruct H3 as [t'].
+      split. unfold transfer.
+      exists (cons (pair ex5 (sse_ev t')) θ'). econstructor; auto.
+      -- admit.
+      -- admit.
+      -- admit.
+      -- eapply inst_ev_ubs with (ub':=t') (t':=t'). 
+        ++ generalize dependent dwl. induction tl; intros. 
+          ** econstructor.
+          ** dependent destruction H1. 
+              eapply inst_ev_ubs with (ub':=t2') (t':=t'); admit.
+        ++ admit. (* inst_weakening *)
+        ++ econstructor; admit.
+        ++ apply ld_sub_refl. admit.
+      -- auto.
   - admit. (* same as previous *)
-  - destruct tl; destruct tl'.
+  - destruct IHla_worklist_reducible as [dwl Hdwl]. destruct Hdwl. 
+    destruct tl; destruct tl'.
     + inversion H0. + inversion H. +inversion H0.
-    + admit.
+    + clear H. clear H0. admit.
   - destruct IHla_worklist_reducible as [dwl [Hdwl_trans Hdwl_red]]. 
     exists (ld_wl_cons_w dwl (ld_w_sub ld_t_int ld_t_int)). split; auto. unfold transfer in *. 
     unfold transfer in Hdwl_trans. destruct Hdwl_trans as [θ Hθ]. 
@@ -50,14 +124,17 @@ Proof.
     + admit.
     + econstructor; eauto.
       econstructor; admit.
-  - (* e_var *) admit.
+  - destruct IHla_worklist_reducible as [dwl [Hdwl_trans Hdwl_red]]. 
+  (* **ex in wl -> ex : t in ss *)
+  admit.
   - (* forall_l *) destruct IHla_worklist_reducible as [dwl [Hdwl_trans Hdwl_red]].
-    unfold transfer in Hdwl_trans. destruct Hdwl_trans as [θ Hθ]. inversion Hθ. 
+    unfold transfer in Hdwl_trans.
+    destruct Hdwl_trans as [θ Hθ]. inversion Hθ. 
     dependent destruction H6. subst.
     exists (ld_wl_cons_w dwl0 (ld_w_sub (ld_t_forall t1') t2')). (* fix this *) split.
     + subst. unfold transfer. exists θ'0. econstructor; eauto.
-      * econstructor. admit.
-      * admit.
+      * admit. 
+      * admit. (* *ss_weakening *)
     + admit.
   - (* forall_r *) admit.
   - (* arrow *) destruct IHla_worklist_reducible as [dwl [Hdwl_trans Hdwl_red]].
@@ -66,8 +143,42 @@ Proof.
     + unfold transfer. exists θ'. eapply inst_wl_sub; eauto.
       econstructor; eauto. econstructor; eauto.
     + admit.
+  - (* -> R *)
+    destruct IHla_worklist_reducible as [dwl [Hdwl_trans Hdwl_red]].
+    unfold transfer in Hdwl_trans.
+    destruct Hdwl_trans as [θ Hθ]. 
+    dependent destruction Hθ.
+    dependent destruction H4.
+    dependent destruction H5.
+    exists (ld_wl_cons_w dwl
+                  (ld_w_sub (ld_t_arrow A0 B0) (ld_t_arrow A1 B1))).
+    split; auto.
+    unfold transfer. exists θ. econstructor.
+    + admit. (* reorder of awl does not change its instantiated awl *)
+    + admit. (* ex still exists in the reordered awl, and should be instantiated to the same type *)
+    + constructor; auto.
+  - (* -> L *)
+  (* exactly same as the previous one*) 
+    destruct IHla_worklist_reducible as [dwl [Hdwl_trans Hdwl_red]].
+    unfold transfer in Hdwl_trans.
+    destruct Hdwl_trans as [θ Hθ]. 
+    dependent destruction Hθ.
+    dependent destruction H4.
+    dependent destruction H5.
+    exists (ld_wl_cons_w dwl
+                (ld_w_sub (ld_t_arrow A0 B0) (ld_t_arrow A1 B1))).
+    split; auto.
+    unfold transfer. exists θ. econstructor.
+    + admit. 
+    + constructor; auto.
+    + admit.
+  - (* EVar L*)
+    admit.
+  - (* EVar L*)
+    admit.
   - destruct IHla_worklist_reducible as [dwl [Hdwl_trans Hdwl_red]].
-    unfold transfer in Hdwl_trans. destruct Hdwl_trans as [θ Hθ]. 
-    exists dwl. split.
-    + unfold transfer. exists θ. econstructor.
+    unfold transfer in Hdwl_trans.
+    destruct Hdwl_trans as [θ Hθ].
+    admit. 
+  - admit.
 Admitted.
